Replace simpl with cbn and rewrite log rep to make automation work manageable - Rest of append_ok post-condition proof

src/ChecksumLog.v
@@ -12,6 +12,7 @@ Require Import Omega.
 Require Import GenSep.
 Require Import PredCrash.
 Require Import Rec.
+Require Import Eqdep_dec.
 
 Import ListNotations.
 Set Implicit Arguments.
@@ -42,12 +43,35 @@ Definition valu_to_header (v : valu) : header.
   exact (Rec.of_word v).
 Defined.
 
+Lemma of_to_header : forall h,
+  valu_to_header (header_to_valu h) = h.
+Proof.
+  intros.
+  destruct h.
+  unfold valu_to_header, header_to_valu.
+  unfold eq_rec_r, eq_rec.
+  rewrite eq_rect_nat_double.
+  rewrite <- (eq_rect_eq_dec eq_nat_dec).
+  repeat rewrite Rec.of_to_id.
+  reflexivity.
+
+  unfold Rec.well_formed.
+  simpl.
+  intuition.
+Qed.
+
+
 Parameter maxlen : addr.
 Definition Header : addr := $0.
 Definition DataStart : addr := $1.
 
 Definition list_prefix A (p l : list A) :=
   firstn (length p) l = p.
+
+Check header_to_valu.
+
+Definition hide_rec p : Prop := p.
+Opaque hide_rec.
 
 (** Log_rep:
   - The current list of values in the log is a prefix of the disk.
@@ -56,16 +80,17 @@ Definition list_prefix A (p l : list A) :=
   Eventually current_length can live in memory **)
 Definition log_rep previous_length vl vdisk hm :
   @pred addr (@weq addrlen) valuset :=
-  (exists h current_length,
-    let header := make_header
+  (exists h current_length header,
+    let header' := make_header
       :=> "previous_length" := ($ previous_length)
       :=> "current_length"  := ($ current_length)
       :=> "checksum"        := h
     in
-    [[ hash_list_rep (rev vl) h hm ]] *
-    [[ length vl = current_length ]] *
-    [[ list_prefix vl vdisk ]] *
-    [[ length vdisk = # (maxlen) ]] *
+    [[ hash_list_rep (rev vl) h hm /\
+        length vl = current_length /\
+        list_prefix vl vdisk /\
+        length vdisk = # (maxlen) ]] *
+    [[ hide_rec (header = header') ]] *
     Header |-> (header_to_valu header, nil) *
     array DataStart (combine vdisk (repeat nil # (maxlen))) $1)%pred.
 
@@ -78,14 +103,14 @@ Definition append T v cs rx : prog T :=
   let header := valu_to_header header_valu in
   let log_pointer := header :-> "current_length" in
   checksum <- Hash (Word.combine v (header :-> "checksum"));
-  cs <- BUFCACHE.write_array DataStart log_pointer $1 v cs;
+  cs <- BUFCACHE.write_array DataStart log_pointer v cs;
   cs <- BUFCACHE.write Header (header_to_valu (
           make_header
             :=> "previous_length" := log_pointer
             :=> "current_length" := log_pointer ^+ $1
             :=> "checksum" := checksum
           )) cs;
-  cs <- BUFCACHE.sync_array DataStart log_pointer $1 cs;
+  cs <- BUFCACHE.sync_array DataStart log_pointer cs;
   cs <- BUFCACHE.sync Header cs;
   rx cs.
 
@@ -99,6 +124,12 @@ Definition truncate T cs rx : prog T :=
           )) cs;
   cs <- BUFCACHE.sync Header cs;
   rx cs.
+
+Ltac unhide_rec :=
+  match goal with
+  | [H: hide_rec _ |- _ ] => inversion H
+  end;
+  subst.
 
 Theorem append_ok : forall v cs,
   {< d previous_length vl,
@@ -117,8 +148,80 @@ Proof.
   pred_apply; cancel.
 
   step.
+  rewrite of_to_header.
+  simpl.
+  step.
+
+  Transparent hide_rec.
+  unhide_rec.
+  rewrite combine_length, repeat_length.
+  rewrite wordToNat_natToWord_bound with (bound:=maxlen); try omega.
+  rewrite min_r; omega.
+
+  step.
+  pred_apply; cancel.
+
   step_idtac.
-Admitted.
+  eauto.
+  pred_apply; cancel_with eauto.
+  unhide_rec.
+  rewrite length_updN, combine_length, repeat_length.
+  rewrite wordToNat_natToWord_bound with (bound:=maxlen); try omega.
+  rewrite min_r; omega.
+
+  step_idtac.
+  cancel_with eauto.
+  pred_apply; cancel_with eauto.
+
+  step_idtac.
+  rewrite <- combine_updN.
+  replace (updN (repeat nil # (maxlen)) # (w1) nil) with (repeat (@nil valu) # (maxlen)).
+  eauto.
+  erewrite selN_eq_updN_eq; eauto.
+  rewrite repeat_selN; auto.
+  unhide_rec.
+  rewrite wordToNat_natToWord_bound with (bound:=maxlen); try omega.
+
+  rewrite rev_unit.
+  solve_hash_list_rep.
+  solve_hash_list_rep.
+  eauto.
+
+  unhide_rec.
+  eapply hashmap_get_subset.
+  rewrite upd_hashmap'_eq. eauto.
+  intuition.
+  unfold hash2, hash_safe in *.
+  rewrite H13 in H17.
+  intuition.
+  contradict_hashmap_get_default H15 hm0.
+  contradict_hashmap_get_default H15 hm0.
+  instantiate (Goal2:=hm0).
+  solve_hashmap_subset.
+
+  unhide_rec.
+  unfold list_prefix in *.
+  rewrite app_length; simpl.
+  rewrite wordToNat_natToWord_bound with (bound := maxlen);
+    try omega.
+  rewrite <- firstn_app_updN_eq.
+  rewrite selN_updN_eq; simpl.
+  congruence.
+  rewrite combine_length, repeat_length.
+  rewrite min_r; omega.
+  omega.
+  rewrite length_updN. omega.
+
+  unfold hide_rec.
+  unhide_rec.
+  rewrite natToWord_plus.
+  unfold hash2.
+  auto.
+
+  all: cancel_with eauto.
+  Grab Existential Variables.
+  auto.
+Qed.
 
 Theorem truncate_ok : forall cs,
   {< d previous_length vl,
@@ -136,7 +239,8 @@ Proof.
   step.
   step.
   step.
-  solve_hash_list_rep.
-  econstructor; eauto.
+  solve_hash_list_rep; eauto.
   unfold list_prefix, firstn; auto.
+  unfold hide_rec.
+  auto.
 Qed.
